AwsCryptographicMaterialProviders/dafny/AwsCryptographyKeyStore/src/HierarchicalVersionUtils.dfy
@@ -7,7 +7,9 @@ module HierarchicalVersionUtils {
 
   import opened Wrappers
   import AtomicPrimitives
-
+  import opened StandardLibrary.UInt
+  import Structure
+  
   method ProvideCryptoClient(
     // Crypto?: Option<AtomicPrimitives.Types.IAwsCryptographicPrimitivesClient> := None
     Crypto?: Option<AtomicPrimitives.AtomicPrimitivesClient> := None
@@ -31,5 +33,32 @@ module HierarchicalVersionUtils {
     // If we create the Crypto Client, it is fresh
     assume {:axiom} fresh(Crypto) && fresh(Crypto.Modifies);
     return Success(Crypto);
+  }
+
+  // unpacks PlainTextTuple (i.e (MD_DIGEST + AES_256 key)) to return MD_DIGEST, AES_256 key
+  function UnpackPlainTextTuple (
+    plainTextTuple: seq<uint8>
+  ) : (Result:(seq<uint8>, seq<uint8>)) 
+  requires |plainTextTuple| == Structure.MD_DIGEST_LENGTH + Structure.AES_256_LENGTH
+  ensures |Result.0| == Structure.MD_DIGEST_LENGTH
+  ensures |Result.1| == Structure.AES_256_LENGTH
+  ensures Result.0 == plainTextTuple[..Structure.MD_DIGEST_LENGTH]
+  ensures Result.1 == plainTextTuple[Structure.MD_DIGEST_LENGTH..]
+  {
+    (plainTextTuple[..Structure.MD_DIGEST_LENGTH], plainTextTuple[Structure.MD_DIGEST_LENGTH..])
+  }
+
+  // packs mdDigest and AES 256 Key into (mdDigest + aes256Key)
+  function PackPlainTextTuple (
+    mdDigest: seq<uint8>, aes256Key: seq<uint8>
+  ) : (Result:(seq<uint8>)) 
+  requires |mdDigest| == Structure.MD_DIGEST_LENGTH
+  requires |aes256Key| == Structure.AES_256_LENGTH
+  ensures |Result| == |mdDigest| + |aes256Key|
+  ensures Result[..Structure.MD_DIGEST_LENGTH] == mdDigest
+  ensures Result[Structure.MD_DIGEST_LENGTH..] == aes256Key
+  ensures Result == mdDigest + aes256Key
+  {
+    (mdDigest + aes256Key)
   }
 }
